Constraint reference parameters.
Reference parameters need to be constraint in two ways:

1. We need to assume the selection path is in range of the current stratification depth. Otherwise we create a logic inconsistency if the reference is read (e.g. that a value both is#Integer and is#Map).
2. We need to assume that a local index is within the current memory range. Otherwise, newly created locals can be aliases with the passed references, which is not possible in Move.

This change adds those assumptions for ref parameters as part of the generated type checking assumptions.

language/move-prover/bytecode-to-boogie/src/spec_translator.rs
@@ -211,7 +211,7 @@ impl<'a> SpecTranslator<'a> {
     /// Translate a dereference.
     fn translate_dref(&mut self, loc: &StorageLocation) -> BoogieExpr {
         let BoogieExpr(s, t) = self.translate_location_as_reference(loc);
-        if let SignatureToken::Reference(sig) = t {
+        if let SignatureToken::Reference(sig) | SignatureToken::MutableReference(sig) = t {
             BoogieExpr(format!("Dereference(m, {})", s), *sig)
         } else {
             self.error(
@@ -412,7 +412,7 @@ impl<'a> SpecTranslator<'a> {
             StorageLocation::AccessPath { base, fields } => {
                 let BoogieExpr(mut res, mut t) = self.translate_location_as_value(base);
                 // If the type of the location is a reference, dref it now.
-                if let SignatureToken::Reference(vt) = t {
+                if let SignatureToken::Reference(vt) | SignatureToken::MutableReference(vt) = t {
                     res = format!("Dereference(m, {})", res);
                     t = *vt;
                 }
@@ -435,7 +435,7 @@ impl<'a> SpecTranslator<'a> {
         match loc {
             StorageLocation::Formal(name) => {
                 let BoogieExpr(s, t) = self.translate_param(name);
-                if let SignatureToken::Reference(_) = t {
+                if let SignatureToken::Reference(_) | SignatureToken::MutableReference(_) = t {
                     BoogieExpr(s, SignatureToken::Reference(Box::new(t)))
                 } else {
                     self.error(
